Lemma/Tensor/DataUnsqueeze/as/Data.lean
@@ -1,9 +1,7 @@
+import Lemma.Bool.SEqCast.of.Eq
 import Lemma.List.ProdInsertIdx.eq.Prod
-import Lemma.Nat.Cast.eq.Mk.of.Lt.Eq
-import Lemma.Vector.EqGetRange
-import Lemma.Vector.SEq.of.All_EqGetS.Eq
-import sympy.tensor.tensor
-open List Vector Nat
+import Lemma.Tensor.DataUnsqueeze.eq.Cast_Data
+open Bool Tensor List
 
 
 @[main]
@@ -15,16 +13,9 @@ private lemma main
 -- imply
   (X.unsqueeze d).data ≃ X.data := by
 -- proof
-  simp [Tensor.unsqueeze]
-  have h_prod := ProdInsertIdx.eq.Prod s d
-  apply SEq.of.All_EqGetS.Eq.fin h_prod
-  intro t
-  have h_t := t.isLt
-  simp [GetElem.getElem]
-  apply congrArg
-  simp [EqGetRange.fin]
-  apply Cast.eq.Mk.of.Lt.Eq
-  assumption
+  rw [DataUnsqueeze.eq.Cast_Data]
+  apply SEqCast.of.Eq
+  apply Prod.eq.ProdInsertIdx
 
 
 -- created on 2025-11-30
